new Lithium

src/Iris/Examples/Lithium.lean
@@ -33,62 +33,41 @@ macro_rules
   | `($a ≫= $args) => `(.bind $a $args)
   | `($a ≫ $args) => `(.bind $a λ _ => $args)
 
-namespace HBind
--- this does not really work
-class HBind (α : outParam (Type u)) (mα : Type v) (nβ : Type w) where
-  hbind : mα → (α → nβ) → nβ
-class HPure (α : outParam (Type u)) (mα : Type v) where
-  hpure : α → mα
-end HBind
-
 namespace Iris.Lithium
-open Lean BI Std HBind
+open Lean BI Std
 
-variable [BI.{u} PROP]
+variable [BI.{u} PROP] {α : Type v} {β : Type w}
 
 structure Atom (α : Type v) where
   ref : α → PROP
 
-structure InExM (α : Type v) where
+structure InEx (α : Type v) where
   body : α → PROP
 
-structure LithiumM (α : Type v) where
+structure Li (α : Type v) where
   run : (α → PROP) → PROP
   mono' E1 E2 : ⊢ run E1 -∗ (∀ a, E1 a -∗ E2 a) -∗ run E2
 
-namespace InExM
+section InEx
 
-variable {α : Type v} {β : Type w}
+def InEx.pure (a : α) : @InEx PROP α :=
+  InEx.mk λ b => iprop(⌜a = b⌝)
 
-def pure (a : α) : @InExM PROP α :=
-  InExM.mk λ b => iprop(⌜a = b⌝)
+def InEx.bind (L1 : @InEx PROP α) (L2 : α → @InEx PROP β) :
+  @InEx PROP β :=
+  InEx.mk λ b => iprop(∃ a, L1.body a ∗ (L2 a).body b)
 
-def bind (L1 : @InExM PROP α) (L2 : α → @InExM PROP β) :
-  @InExM PROP β :=
-  InExM.mk λ b => iprop(∃ a, L1.body a ∗ (L2 a).body b)
-
-instance : Monad (@InExM PROP) where
+instance : Monad (@InEx PROP) where
   pure := .pure
   bind := .bind
 
-instance : HBind α (@InExM PROP α) (@InExM PROP β) where
-  hbind := .bind
-instance : HPure α (@InExM PROP α) where
-  hpure := .pure
+def atom (A : @Atom PROP α) : @InEx PROP α := InEx.mk A.ref
+def own (P : PROP) : @InEx PROP Unit := .mk λ _ => iprop(P)
+def prop (P : Prop) : @InEx PROP Unit := own iprop(⌜P⌝)
 
-def atom (A : @Atom PROP α) : @InExM PROP α := InExM.mk A.ref
-def own (P : PROP) : @InExM PROP Unit := .mk λ _ => iprop(P)
-def ownP (P : PROP) : @InExM PROP PUnit := .mk λ _ => iprop(P)
-def prop (P : Prop) : @InExM PROP Unit := own iprop(⌜P⌝)
-def propP (P : Prop) : @InExM PROP PUnit := ownP iprop(⌜P⌝)
+end InEx
 
-end InExM
-
-namespace LithiumM
-
-variable {α : Type v} {β : Type w}
-
-def pure (a : α) : @LithiumM PROP _ α := {
+def Li.pure (a : α) : @Li PROP _ α := {
   run E := E a
   mono' E1 E2 := by
     dsimp
@@ -97,8 +76,8 @@ def pure (a : α) : @LithiumM PROP _ α := {
     iassumption
 }
 
-def bind (G1 : @LithiumM PROP _ α) (G2 : α → @LithiumM PROP _ β) :
-  @LithiumM PROP _ β := {
+def Li.bind (G1 : @Li PROP _ α) (G2 : α → @Li PROP _ β) :
+  @Li PROP _ β := {
   run E := G1.run (λ a => (G2 a).run E)
   mono' E1 E2 := by
     dsimp
@@ -106,19 +85,17 @@ def bind (G1 : @LithiumM PROP _ α) (G2 : α → @LithiumM PROP _ β) :
     sorry
 }
 
-instance : Monad (@LithiumM PROP _) where
+instance : Monad (@Li PROP _) where
   pure := .pure
   bind := .bind
 
-instance : HBind α (@LithiumM PROP _ α) (@LithiumM PROP _ β) where
-  hbind := .bind
-instance : HPure α (@LithiumM PROP _ α) where
-  hpure := .pure
+def exhaleR (L : @InEx PROP α) (E : α → PROP) : PROP :=
+  iprop(∃ a, L.body a ∗ E a)
 
-def exhale (L : @InExM PROP α) : @LithiumM PROP _ α := {
-  run E := iprop(∃ a, L.body a ∗ E a)
+def exhale (L : @InEx PROP α) : @Li PROP _ α := {
+  run := exhaleR L
   mono' E1 E2 := by
-    dsimp
+    dsimp [exhaleR]
     iintro ⟨a, HL, HE⟩ Hwand
     iexists a
     isplit l [HL]
@@ -127,53 +104,66 @@ def exhale (L : @InExM PROP α) : @LithiumM PROP _ α := {
     iassumption
 }
 
-def inhale (L : @InExM PROP α) : @LithiumM PROP _ α := {
-  run E := iprop(∀ a, L.body a -∗ E a)
+def inhaleR (L : @InEx PROP α) (E : α → PROP) : PROP :=
+  iprop(∀ a, L.body a -∗ E a)
+
+def inhale (L : @InEx PROP α) : @Li PROP _ α := {
+  run := inhaleR L
   mono' E1 E2 := by
-    dsimp
+    dsimp [inhaleR]
     iintro HE Hwand a HL
     ispecialize HE HL
     ispecialize Hwand HE
     iassumption
 }
 
-def all (α : Type v) : @LithiumM PROP _ α := {
-  run E := iprop(∀ a, E a)
+def allR (α : Type v) (E : α → PROP) : PROP :=
+  iprop(∀ a, E a)
+
+def all (α : Type v) : @Li PROP _ α := {
+  run := allR α
   mono' E1 E2 := by
-    dsimp
+    dsimp [allR]
     iintro HE Hwand a
     ispecialize HE a
     ispecialize Hwand HE
     iassumption
 }
 
-def done : @LithiumM PROP _ α := {
-  run E := iprop(True)
+def doneR : PROP := iprop(True)
+
+def done : @Li PROP _ α := {
+  run E := doneR
   mono' E1 E2 := by
-    dsimp
+    dsimp [doneR]
     iintro HE Hwand
     iassumption
 }
 
-def lif (P : Prop) (G1 G2 : @LithiumM PROP _ α) : @LithiumM PROP _ α := {
-  run E := iprop((⌜P⌝ -∗ G1.run E) ∧ (⌜¬P⌝ -∗ G2.run E))
+def lifR (P : Prop) (E1 E2 : PROP) : PROP :=
+  iprop((⌜P⌝ -∗ E1) ∧ (⌜¬P⌝ -∗ E2))
+
+def lif (P : Prop) (G1 G2 : @Li PROP _ α) : @Li PROP _ α := {
+  run E := lifR P (G1.run E) (G2.run E)
   mono' E1 E2 := by
     dsimp
     iintro HE Hwand
     sorry
 }
 
-def dsimp {α : Type _} [BI PROP] (_ : Lean.Name) (a : α) : @LithiumM PROP _ α := {
-  run E := E a
+def dsimpR {α : Type _} [BI PROP] (_ : Lean.Name) (a : α) (E : α → PROP) : PROP := E a
+
+def dsimp {α : Type _} [BI PROP] (n : Lean.Name) (a : α) : @Li PROP _ α := {
+  run := dsimpR n a
   mono' E1 E2 := by
-    simp
+    simp [dsimpR]
     sorry
 }
 
 def empty : Empty → PROP := λ e => nomatch e
-def emptyP : PEmpty → PROP := λ e => nomatch e
 
-def dualizing (G : @LithiumM PROP _ Empty) : @LithiumM PROP _ Unit := {
+-- TODO: add R variant
+def dualizing (G : @Li PROP _ Empty) : @Li PROP _ Unit := {
   run E := iprop(G.run empty -∗ E ⟨⟩)
   mono' E1 E2 := by
     dsimp
@@ -183,125 +173,77 @@ def dualizing (G : @LithiumM PROP _ Empty) : @LithiumM PROP _ Unit := {
     iassumption
 }
 
-def dualizingP (G : @LithiumM PROP _ PEmpty) : @LithiumM PROP _ PUnit := {
-  run E := iprop(G.run emptyP -∗ E ⟨⟩)
-  mono' E1 E2 := by
-    dsimp
-    iintro HE Hwand HG
-    ispecialize HE HG
-    ispecialize Hwand HE
-    iassumption
-}
+---- TODO: What are good precedences?
+--notation:35 G:36 " ⇓ " E:35 => run G E
+--notation:35 G:36 " ⇓ " "!" => run G empty
 
--- TODO: What are good precedences?
-notation:35 G:36 " ⇓ " E:35 => run G E
-notation:35 G:36 " ⇓ " "!" => run G empty
-
-def entails (G1 G2 : @LithiumM PROP _ α) : Prop :=
-  ∀ E, G1.run E ⊢ G2.run E
+--def entails (G1 G2 : @Li PROP _ α) : Prop :=
+--  ∀ E, G1.run E ⊢ G2.run E
 
 --notation:25 G1:29 ":-" G2:25 => (entails G2 G1)
 --set_option quotPrecheck false in -- TODO: Why is this necessary?
 --notation:25 G1:29 ":-" G2:25 => (∀ E, (G2 ⇓ E ⊢ G1 ⇓ E))
 notation:25 P:29 "⊣" Q:25 => (Q ⊢ P)
+set_option quotPrecheck false in -- TODO: Why is this necessary?
+notation:25 P:29 ":-" Q:25 => (∀ E, Li.run Q E ⊢ P E)
 
 --notation:25 G1:29 ":-" G2:25 => (run! G2 ⊢ run! G1)
 
-end LithiumM
+-- @[irun]
+-- theorem run_bind (G1 : @Li PROP _ α) (G2 : α → Li β)
+--   (E : β → PROP) :
+--    G1.bind G2 ⇓ E ⊣ (G1 ⇓ λ b => G2 b ⇓ E) := by
+--     simp [Li.bind, Li.run, Li.run]
+
+-- @[irun]
+-- theorem run_pure (a : α) (E : α → PROP) :
+--    .pure a ⇓ E ⊣ E a := by
+--     simp [Li.pure, Li.run, Li.run]
+
+attribute [irun_preprocess] inhale exhale Lithium.done Li.run Li.bind
 
 @[irun]
-theorem run_bind (G1 : @LithiumM PROP _ α) (G2 : α → LithiumM β)
-  (E : β → PROP) :
-   G1.bind G2 ⇓ E ⊣ (G1 ⇓ λ b => G2 b ⇓ E) := by
-    simp [LithiumM.bind, LithiumM.run, LithiumM.run]
-
-@[irun]
-theorem run_pure (a : α) (E : α → PROP) :
-   .pure a ⇓ E ⊣ E a := by
-    simp [LithiumM.pure, LithiumM.run, LithiumM.run]
-
-@[irun]
-theorem exhale_bind (L1 : @InExM PROP α) (L2 : α → InExM β) E :
-  .exhale (L1.bind L2) ⇓ E ⊣
-    LithiumM.exhale L1 ⇓ λ a => LithiumM.exhale (L2 a) ⇓ E := by
-    dsimp [bind, LithiumM.bind, LithiumM.exhale, LithiumM.run, InExM.bind, LithiumM.run]
+theorem exhale_bind (L1 : @InEx PROP α) (L2 : α → InEx β) :
+  exhaleR (L1.bind L2) :-
+    ((exhale L1).bind λ a => exhale (L2 a)) := by
+    dsimp [exhaleR, InEx.bind]
     sorry
 
 @[irun]
-theorem inhale_bind (L1 : @InExM PROP α) (L2 : α → InExM β) E :
-  .inhale (L1.bind L2) ⇓ E ⊣
-   LithiumM.inhale L1 ⇓ λ a => .inhale (L2 a) ⇓ E := by
-    dsimp [bind, LithiumM.bind, LithiumM.inhale, LithiumM.run, InExM.bind]
+theorem inhale_bind (L1 : @InEx PROP α) (L2 : α → InEx β) E :
+  inhaleR (L1.bind L2) E ⊣
+   inhaleR L1 λ a => inhaleR (L2 a) E := by
+    dsimp [inhaleR, InEx.bind]
     sorry
 
 @[irun]
 theorem exhale_pure (a : α) E :
-  .exhale (PROP:=PROP) (.pure a) ⇓ E ⊣ E a := by
-    dsimp [bind, LithiumM.pure, LithiumM.exhale, LithiumM.run, InExM.pure]
+  exhaleR (PROP:=PROP) (.pure a) E ⊣ E a := by
+    dsimp [exhaleR, InEx.pure]
     sorry
 
 @[irun]
 theorem inhale_pure (a : α) E :
-  .inhale (PROP:=PROP) (.pure a) ⇓ E ⊣ E a := by
-    dsimp [bind, LithiumM.pure, LithiumM.inhale, LithiumM.run, InExM.pure]
+  inhaleR (PROP:=PROP) (.pure a) E ⊣ E a := by
+    dsimp [inhaleR, InEx.pure]
     sorry
 
 
-def test_inexP (A : @Atom PROP (ULift.{u} Nat)) : @InExM PROP (ULift.{u} Bool) := do
-  let n ← .atom A
-  .ownP (A.ref n)
-  return ULift.up (n.down == 1)
-
 set_option pp.universes true
 
-def test_inex (A : @Atom PROP Nat) : @InExM PROP Bool :=
-  .atom A ≫= λ n =>
-  .own (A.ref n) ≫
+def test_inex (A : @Atom PROP Nat) : @InEx PROP Bool :=
+  atom A ≫= λ n =>
+  own (A.ref n) ≫
   .pure (n == 1)
 
-def test_inexh (A : @Atom PROP Nat) : @InExM PROP Bool :=
-  HBind.hbind (InExM.atom A) λ n =>
-  HBind.hbind (InExM.own (A.ref n)) λ _ =>
-  InExM.pure (n == 1)
-
-
-def test_lithiumP (A : @Atom PROP (ULift.{u} Nat)) : @LithiumM PROP _ (ULift.{u} Bool) := do
-  let b ← .exhale do
-    let n ← .atom A
-    return ULift.up (n.down == 1)
-  .inhale do
-    let n ← .atom A
-    .propP (b.down = (n.down == 1))
-    return ULift.up true
-
-
-def test_lithium (A : @Atom PROP Nat) : @LithiumM PROP _ Bool := do
-  (LithiumM.exhale <|
-    .atom A ≫= λ n =>
+def test_lithium (A : @Atom PROP Nat) : @Li PROP _ Bool := do
+  (exhale <|
+    atom A ≫= λ n =>
     .pure (n == 1)) ≫= λ b =>
-  LithiumM.inhale <|
-    .atom A ≫= λ n =>
-    .prop (b = (n == 1)) ≫
+  inhale <|
+    atom A ≫= λ n =>
+    prop (b = (n == 1)) ≫
     .pure true
-
--- set_option pp.universes true
-
--- #check InExM.instHBind
--- #check LithiumM.instHBind
-
-/--
-error: typeclass instance problem is stuck, it is often due to metavariables
-  HBind.{0, u, u} Bool (LithiumM.{u, 0} Bool) (LithiumM.{u, 0} Bool)
--/
-#guard_msgs in
-def test_lithiumH (A : @Atom PROP Nat) : @LithiumM PROP _ Bool := do
-  HBind.hbind (LithiumM.exhale.{u} (α:=Bool) <|
-    HBind.hbind (InExM.atom A) λ n =>
-    HPure.hpure (n == 1)) λ b =>
-  LithiumM.inhale <|
-    HBind.hbind (InExM.atom A) λ n =>
-    HBind.hbind (InExM.prop (b = (n == 1))) λ _=>
-    HPure.hpure true
 
 end Iris.Lithium
 
@@ -310,15 +252,15 @@ open Lean Elab Tactic Meta Qq BI Std Lithium
 
 theorem inhale_own_tac [BI PROP] {P A : PROP} (E : Unit → PROP)
   (h : P ∗ A ⊢ E ())
- : P ⊢ (LithiumM.inhale (.own A)) ⇓ E := by
-    simp [LithiumM.run, LithiumM.inhale, InExM.own, InExM.body]
+ : P ⊢ (inhaleR (own A)) E := by
+    simp [inhaleR, own]
     sorry
 
-@[irun_tac (LithiumM.inhale (InExM.own _)) ⇓ _]
+@[irun_tac (inhaleR (own _)) _]
 def irunInhaleOwn : IRunTacticType := fun goal => do profileitM Exception "irunIntro" (← getOptions) do
   let g ← instantiateMVars <| ← goal.getType
   let some { prop, bi, e, hyps, goal:=G } := parseIrisGoal? g | throwError "not in proof mode"
-  let ~q(LithiumM.run (LithiumM.inhale (.own $A)) $E) := G | return none
+  let ~q(inhaleR (own $A) $E) := G | return none
   let ident ← `(binderIdent| _)
   let (b, A') := if A.isAppOfArity ``intuitionistically 3 then
       (q(true), A.getArg! 3)
@@ -338,14 +280,14 @@ def irunInhaleOwn : IRunTacticType := fun goal => do profileitM Exception "irunI
 theorem cancel [BI PROP] {p : Bool} {P P' A : PROP} {E}
   (hP : P ⊣⊢ P' ∗ □?p A)
   (h : P' ⊢ E ())
- : P ⊢ LithiumM.exhale (.own A) ⇓ E := by
+ : P ⊢ exhaleR (own A) E := by
    sorry
 
-@[irun_tac LithiumM.exhale (InExM.own _) ⇓ _]
+@[irun_tac exhaleR (own _) _]
 def irunCancel : IRunTacticType := fun goal => do profileitM Exception "irunCancel" (← getOptions) do
   let g ← instantiateMVars <| ← goal.getType
   let some { prop, bi, hyps, goal:=G } := parseIrisGoal? g | throwError "not in proof mode"
-  let ~q(LithiumM.exhale (.own $A) ⇓ $E) := G | return none
+  let ~q(exhaleR (own $A) $E) := G | return none
   let some ⟨_inst, P', hyps, out, ty, b, _, pf⟩ ←
     hyps.removeG false fun _ _ _ ty => do
       -- logInfo m!"ty: ${ty}, A: ${A}"
@@ -359,34 +301,31 @@ def irunCancel : IRunTacticType := fun goal => do profileitM Exception "irunCanc
   goal.assign pf
   return .some ([m.mvarId!], [])
 
-theorem done_tac {α : Type _} [BI PROP] (P : PROP) (E : α → PROP)
- : P ⊢ LithiumM.done ⇓ E := pure_intro .intro
+theorem done_tac [BI PROP] (P : PROP)
+ : P ⊢ doneR := pure_intro .intro
 
 --set_option pp.universes true
 
-@[irun_tac LithiumM.done ⇓ _]
+@[irun_tac doneR]
 def irunDone : IRunTacticType := fun goal => do profileitM Exception "irunTrue" (← getOptions) do
   let g ← instantiateMVars <| ← goal.getType
   let some { prop:=prop, bi:=bi, hyps:=_, e, goal:=G } := parseIrisGoal? g | throwError "not in proof mode"
-  match_expr G with
-  | LithiumM.run _ _ α G E =>
-    let .true := G.isAppOfArity ``LithiumM.done 3 | return none
-    let pf := mkApp5 (.const ``done_tac G.getAppFn.constLevels!) prop α bi e E
-    goal.assign pf
-    return .some ([], [])
-  | _ => return none
+  let .true := G.isAppOfArity ``doneR 2 | return none
+  let pf := mkApp3 (.const ``done_tac G.getAppFn.constLevels!) prop bi e
+  goal.assign pf
+  return .some ([], [])
 
 
-theorem lif_true {α : Type _} [BI PROP] {cond} {P : PROP} (G1 : LithiumM α) G2 E
+theorem lif_true [BI PROP] {cond} {P : PROP} (E1 E2 : PROP)
   (h1 : cond)
-  (h2 : P ⊢ G1 ⇓ E)
- : P ⊢ .lif cond G1 G2 ⇓ E :=
+  (h2 : P ⊢ E1)
+ : P ⊢ lifR cond E1 E2 :=
    sorry
 
-theorem lif_false {α : Type _} [BI PROP] {cond} {P : PROP} (G1 : LithiumM α) G2 E
+theorem lif_false [BI PROP] {cond} {P : PROP} (E1 E2 : PROP)
   (h1 : ¬ cond)
-  (h2 : P ⊢ G2 ⇓ E)
- : P ⊢ .lif cond G1 G2 ⇓ E :=
+  (h2 : P ⊢ E2)
+ : P ⊢ lifR cond E1 E2 :=
    sorry
 
 syntax "istepsolve" : tactic
@@ -395,18 +334,18 @@ macro_rules
 --macro_rules
 --  | `(tactic|istepsolve) => `(tactic|solve| simp)
 
-@[irun_tac LithiumM.lif _ _ _ ⇓ _]
+@[irun_tac lifR _ _ _]
 def irunLif : IRunTacticType := fun goal => do profileitM Exception "irunLif" (← getOptions) do
   let g ← instantiateMVars <| ← goal.getType
   let some { prop, bi, e, hyps, goal:=G } := parseIrisGoal? g | throwError "not in proof mode"
-  let ~q(LithiumM.lif $cond $G1 $G2 ⇓ $E) := G | return none
+  let ~q(lifR $cond $E1 $E2) := G | return none
 
   let mcond : Q($cond) ← mkFreshExprSyntheticOpaqueMVar cond
   try
     let _ ← evalTacticAtRaw (← `(tactic|istepsolve)) mcond.mvarId!
-    let m : Q($e ⊢ $G1 ⇓ $E) ← mkFreshExprSyntheticOpaqueMVar <|
-      IrisGoal.toExpr { prop, bi, hyps := hyps, goal := q($G1 ⇓ $E) }
-    let pf := q(lif_true $G1 $G2 $E $mcond $m)
+    let m : Q($e ⊢ $E1) ← mkFreshExprSyntheticOpaqueMVar <|
+      IrisGoal.toExpr { prop, bi, hyps := hyps, goal := E1 }
+    let pf := q(lif_true $E1 $E2 $mcond $m)
     goal.assign pf
     return .some ([m.mvarId!], [])
   catch _ => pure ()
@@ -414,23 +353,22 @@ def irunLif : IRunTacticType := fun goal => do profileitM Exception "irunLif" (�
   let mnegcond : Q(¬$cond) ← mkFreshExprSyntheticOpaqueMVar q(¬ $cond)
   try
     let _ ← evalTacticAt (← `(tactic|istepsolve)) mnegcond.mvarId!
-    let m : Q($e ⊢ $G2 ⇓ $E) ← mkFreshExprSyntheticOpaqueMVar <|
-      IrisGoal.toExpr { prop, bi, hyps := hyps, goal := q($G2 ⇓ $E) }
-    let pf := q(lif_false $G1 $G2 $E $mnegcond $m)
+    let m : Q($e ⊢ $E2) ← mkFreshExprSyntheticOpaqueMVar <|
+      IrisGoal.toExpr { prop, bi, hyps := hyps, goal := E2 }
+    let pf := q(lif_false $E1 $E2 $mnegcond $m)
     goal.assign pf
     return .some ([m.mvarId!], [])
   catch _ => pure ()
 
   throwError "Cannot solve either side of lif"
 
-@[irun_tac LithiumM.dsimp _ _ ⇓ _]
+@[irun_tac dsimpR _ _ _]
 def irunSimp : IRunTacticType := fun goal => do profileitM Exception "irunSimp" (← getOptions) do
   let g ← instantiateMVars <| ← goal.getType
   let some ig := parseIrisGoal? g | throwError "not in proof mode"
   let { prop:=_, bi:=_, e:=_, hyps:=_, goal:=G } := ig
 
-  let_expr LithiumM.run _ _ _ G E := G | return none
-  let_expr LithiumM.dsimp _ _ _ n e := G | return none
+  let_expr dsimpR _ _ _ n e E := G | return none
   let n : Name ← reduceEval n
   let ⟨e_new, _⟩ ← goal.withContext (dsimpWithExt n e)
   let g' := {ig with goal := Expr.beta E #[e_new]}.toExpr
@@ -441,54 +379,37 @@ section test
 variable {u} [BI.{u} PROP]
 
 theorem test1 (P : Nat → PROP) (Q : PROP) :
-  ⊢ (.inhale (.own Q) ≫
-      .inhale (.own (P 1)) ≫
-      .inhale (.own (P 2)) ≫
-      .inhale (.own iprop(⌜1 = 1⌝)) ≫
-      .exhale (.own (P 1) ≫ .own (P 2)) ≫
-      .exhale (.own Q) ≫
-   .done) ⇓ ! := by
+  ⊢ ((inhale (own Q)).bind λ _ =>
+      inhale (own (P 1)) ≫
+      inhale (own (P 2)) ≫
+      inhale (own iprop(⌜1 = 1⌝)) ≫
+      exhale (own (P 1) ≫ own (P 2)) ≫
+      exhale (own Q) ≫
+     done).run empty := by
      istart
+     simp [irun_preprocess]
      irun ∞
 
 
 theorem test_intro_cancel (P G : PROP) :
-  ⊢ .inhale (.own P ≫ .own G) ⇓ λ _ =>
-     .exhale (.own G) ⇓ λ _ =>
-     .done ⇓ ! := by
+  ⊢ (inhale ((own P) ≫ own G)).run λ _ =>
+     (exhale (own G)).run λ _ =>
+     done.run empty := by
     istart
+    simp [irun_preprocess]
     irun 1
     irun 1
     irun 1
     irun 1
     irun 1
-
-
---set_option profiler true in
---set_option profiler.threshold 1 in
-set_option maxRecDepth 30000 in
-#time theorem proof_cancel_2 (P : Nat → PROP) :
-  ⊢ (List.foldl (λ G n => LithiumM.bind (.inhale (.own (P n))) λ _ => G)
-    (List.foldl (λ G n => LithiumM.bind (.exhale (.own (P n))) λ _ => G) .done (
-    -- List.reverse makes cancellation basically instant
-    -- List.reverse
-    (List.range 2)))
-    (List.range 2)) ⇓ !
-:=
-  by
-    dsimp [List.foldl, List.range, List.range.loop, List.reverse]
-    istart
-    -- set_option trace.profiler true in
-    -- set_option trace.profiler.threshold 1 in
-    irun ∞
 
 --set_option profiler true in
 --set_option profiler.threshold 1 in
 set_option maxRecDepth 30000 in
 #time theorem proof_cancel_3 (P : Nat → PROP) :
-  ⊢ (List.foldl (λ G n => LithiumM.inhale (.own (P n)) ⇓ λ _ => G)
-    (List.foldl (λ G n => LithiumM.exhale (.own (P n)) ⇓ λ _ => G)
-      (.done ⇓ !) (
+  ⊢ (List.foldl (λ G n => inhaleR (own (P n)) λ _ => G)
+    (List.foldl (λ G n => exhaleR (own (P n)) λ _ => G)
+      (doneR) (
     -- List.reverse makes cancellation basically instant
     -- List.reverse
     (List.range 2)))
@@ -497,10 +418,9 @@ set_option maxRecDepth 30000 in
   by
     dsimp [List.foldl, List.range, List.range.loop, List.reverse]
     istart
-    -- set_option trace.profiler true in
+    set_option trace.profiler true in
     -- set_option trace.profiler.threshold 1 in
-    -- irun ∞
-    sorry
+    irun ∞
 
 end test
 
@@ -511,37 +431,19 @@ open Lang Lithium
 
 variable {u} [BI.{u} PROP]
 
-theorem wp_wand e (P1 P2 : Val -> PROP) :
-  ⊢ wp e P1 -∗ (∀ v, P1 v -∗ P2 v) -∗ wp e P2
-  := by sorry
-
-
 /- Proof automation begins here -/
 
-def expr_ok (e : Exp) : @LithiumM PROP _ Val := {
-  run := wp e
+def expr_okR := @wp PROP _
+
+@[irun_preprocess]
+def expr_ok (e : Exp) : @Li PROP _ Val := {
+  run := expr_okR e
   mono' := wp_wand e
 }
 
-def expr_okP (e : Exp) : @LithiumM PROP _ (ULift.{u} Val) := {
-  run E := wp e (λ v => E (ULift.up v))
-  mono' := by sorry
-}
-
-/- problem: Monad is not fully universe polymorphic -/
-def fn_specP (v : Val) (G : Val → @LithiumM PROP _ (Val → @LithiumM PROP _ PEmpty)) : PROP :=
-  iprop(∀ (E : ULift.{u} Val → PROP) va,
-  (do
-    let L' : Val → LithiumM PEmpty ← G va
-    let vr ← .all (ULift.{u} Val)
-    LithiumM.dualizingP (L' vr.down)
-    return vr) ⇓ E
-  -∗
-  wp (.app (.val v) (.val va)) λ v => E (ULift.up v))
-
 -- set_option pp.universes true
-
-def fn_spec (v : Val) (G : Val → @LithiumM PROP _ (Val → @LithiumM PROP _ Empty)) : PROP :=
+/-
+def fn_spec (v : Val) (G : Val → @Li PROP _ (Val → @Li PROP _ Empty)) : PROP :=
   iprop(∀ E va,
   (.bind (G va) λ L' =>
    .bind (.all Val) λ vr =>
@@ -549,28 +451,41 @@ def fn_spec (v : Val) (G : Val → @LithiumM PROP _ (Val → @LithiumM PROP _ Em
    .pure vr) ⇓ E
   -∗
   wp (.app (.val v) (.val va)) E)
+-/
 
-def nat_ok (v : Val) : @LithiumM PROP _ Nat := {
-  run E := iprop(∃ n, ⌜v = .nat n⌝ ∗ E n)
+def nat_okR (v : Val) (E : Nat → PROP) : PROP :=
+  iprop(∃ n, ⌜v = .nat n⌝ ∗ E n)
+
+@[irun_preprocess]
+def nat_ok (v : Val) : @Li PROP _ Nat := {
+  run := nat_okR v
   mono' E1 E2 := by sorry
 }
 
-def recv_ok (v : Val) : @LithiumM PROP _ (String × String × Exp) := {
-  run E := iprop(∃ f x e, ⌜v = .recv f x e⌝ ∗ E (f, x, e))
+def recv_okR (v : Val) (E : String → String → Exp → PROP) : PROP :=
+  iprop(∃ f x e, ⌜v = .recv f x e⌝ ∗ E f x e)
+
+@[irun_preprocess]
+def recv_ok (v : Val) : @Li PROP _ (String × String × Exp) := {
+  run E := recv_okR v λ f x e => E (f, x, e)
   mono' E1 E2 := by sorry
 }
 
-def subst_ok (x : String) (v : Val) (e : Exp) : @LithiumM PROP _ Exp := {
-  run E := E (subst x v e)
+def subst_okR (x : String) (v : Val) (e : Exp) (E : Exp → PROP) : PROP :=
+  E (subst x v e)
+
+@[irun_preprocess]
+def subst_ok (x : String) (v : Val) (e : Exp) : @Li PROP _ Exp := {
+  run := subst_okR x v e
   mono' E1 E2 := by
-    simp
+    simp [subst_okR]
     sorry
 }
 
 @[irun]
-theorem nat_ok_nat (n : Nat) (E : Nat → PROP) :
-  nat_ok (.nat n) ⇓ E ⊣ E n := by
-  dsimp [nat_ok, LithiumM.run, LithiumM.run]
+theorem nat_okR_nat (n : Nat) (E : Nat → PROP) :
+  nat_okR (.nat n) E ⊣ E n := by
+  dsimp [nat_okR]
   iintro HP
   iexists _
   isplit
@@ -579,9 +494,9 @@ theorem nat_ok_nat (n : Nat) (E : Nat → PROP) :
   · iassumption
 
 @[irun]
-theorem recv_ok_rec f x e (E : (String × String × Exp) -> PROP) :
-  recv_ok (.recv f x e) ⇓ E ⊣ E (f, x, e) := by
-  dsimp [recv_ok, LithiumM.run, LithiumM.run]
+theorem recv_okR_rec f x e (E : String → String → Exp -> PROP) :
+  recv_okR (.recv f x e) E ⊣ E f x e := by
+  dsimp [recv_okR]
   iintro HP
   iexists _
   iexists _
@@ -592,77 +507,73 @@ theorem recv_ok_rec f x e (E : (String × String × Exp) -> PROP) :
   · iassumption
 
 @[irun]
-theorem expr_ok_val v (E : Val -> PROP) :
-  expr_ok (.val v) ⇓ E ⊣ E v := by sorry
+theorem expr_okR_val v (E : Val -> PROP) :
+  expr_okR (.val v) E ⊣ E v := by sorry
 
 @[irun]
-theorem expr_ok_plus e1 e2 (E : Val -> PROP) :
-  expr_ok (Exp.binop e1 .plus e2) ⇓ E ⊣
-   expr_ok e1 ⇓ λ v1 =>
-   expr_ok e2 ⇓ λ v2 =>
-   nat_ok v1 ⇓ λ n1 =>
-   nat_ok v2 ⇓ λ n2 =>
-   .dsimp `irun_simp (n1 + n2) ⇓ λ n =>
+theorem expr_okR_plus e1 e2 (E : Val -> PROP) :
+  expr_okR (Exp.binop e1 .plus e2) E ⊣
+   expr_okR e1 λ v1 =>
+   expr_okR e2 λ v2 =>
+   nat_okR v1 λ n1 =>
+   nat_okR v2 λ n2 =>
+   dsimpR `irun_simp (n1 + n2) λ n =>
    E (.nat n) := by sorry
 
 @[irun]
-theorem expr_ok_minus e1 e2 (E : Val -> PROP) :
-  expr_ok (Exp.binop e1 .minus e2) ⇓ E ⊣
-   expr_ok e1 ⇓ λ v1 =>
-   expr_ok e2 ⇓ λ v2 =>
-   nat_ok v1 ⇓ λ n1 =>
-   nat_ok v2 ⇓ λ n2 =>
-   .dsimp `irun_simp (n1 - n2) ⇓ λ n =>
+theorem expr_okR_minus e1 e2 (E : Val -> PROP) :
+  expr_okR (Exp.binop e1 .minus e2) E ⊣
+   expr_okR e1 λ v1 =>
+   expr_okR e2 λ v2 =>
+   nat_okR v1 λ n1 =>
+   nat_okR v2 λ n2 =>
+   dsimpR `irun_simp (n1 - n2) λ n =>
    E (.nat n) := by sorry
 
 @[irun]
-theorem expr_ok_eq e1 e2 (E : Val -> PROP) :
-  expr_ok (Exp.binop e1 .eq e2) ⇓ E ⊣
-   expr_ok e1 ⇓ λ v1 =>
-   expr_ok e2 ⇓ λ v2 =>
-   nat_ok v1 ⇓ λ n1 =>
-   nat_ok v2 ⇓ λ n2 =>
-   .dsimp `irun_simp (if n1 == n2 then 1 else 0) ⇓ λ n =>
+theorem expr_okR_eq e1 e2 (E : Val -> PROP) :
+  expr_okR (Exp.binop e1 .eq e2) E ⊣
+   expr_okR e1 λ v1 =>
+   expr_okR e2 λ v2 =>
+   nat_okR v1 λ n1 =>
+   nat_okR v2 λ n2 =>
+   dsimpR `irun_simp (if n1 == n2 then 1 else 0) λ n =>
    E (.nat n) := by sorry
 
 @[irun]
-theorem expr_ok_rec f x e (E : Val -> PROP) :
-  expr_ok (.rece f x e) ⇓ E ⊣ E (.recv f x e) := by sorry
+theorem expr_okR_rec f x e (E : Val -> PROP) :
+  expr_okR (.rece f x e) E ⊣ E (.recv f x e) := by sorry
 
 @[irun]
-theorem expr_ok_app e1 e2 (E : Val -> PROP) :
-  expr_ok (.app e1 e2) ⇓ E ⊣
-   expr_ok e2 ⇓ λ v2 =>
-   expr_ok e1 ⇓ λ v1 =>
-   recv_ok v1 ⇓ λ ⟨f, x, e'⟩ =>
-   subst_ok x v2 e' ⇓ λ e =>
-   subst_ok f (.recv f x e') e ⇓ λ e =>
-   expr_ok e ⇓ E := by sorry
+theorem expr_okR_app e1 e2 (E : Val -> PROP) :
+  expr_okR (.app e1 e2) E ⊣
+   expr_okR e2 λ v2 =>
+   expr_okR e1 λ v1 =>
+   recv_okR v1 λ f x e' =>
+   subst_okR x v2 e' λ e =>
+   subst_okR f (.recv f x e') e λ e =>
+   expr_okR e E := by sorry
 
 @[irun]
-theorem expr_ok_if e1 e2 e3 (E : Val -> PROP) :
-  (expr_ok e1 ⇓ λ v1 =>
-   nat_ok v1 ⇓ λ n1 =>
-   LithiumM.lif (n1 ≠ 0) (expr_ok e2) (expr_ok e3) ⇓ E) ⊢
-  expr_ok (.ife e1 e2 e3) ⇓ E := by sorry
+theorem expr_okR_if e1 e2 e3 E :
+  (expr_okR (PROP:=PROP) e1 λ v1 =>
+   nat_okR v1 λ n1 =>
+   lifR (n1 ≠ 0) (expr_okR e2 E) (expr_okR e3 E)) ⊢
+  expr_okR (.ife e1 e2 e3) E := by sorry
 
 
 section
 open Lean Elab Tactic Meta Qq BI Std ProofMode
 
-@[irun_tac subst_ok _ _ _ ⇓  _]
+@[irun_tac subst_okR _ _ _ _]
 def irunSubst : IRunTacticType := fun goal => do profileitM Exception "irunSubst" (← getOptions) do
   let g ← instantiateMVars <| ← goal.getType
   let some ig := parseIrisGoal? g | throwError "not in proof mode"
   let { prop:=_, bi:=_, e:=_, hyps:=_, goal:=G } := ig
 
-  let .true := G.isAppOfArity ``LithiumM.run 5 | return none
-  let G' := G.getArg! 3
-  let E := G.getArg! 4
-  let .true := G'.isAppOfArity ``subst_ok 5 | return none
-  let .lit (.strVal x) := G'.getArg! 2 | return none
-  let v := G'.getArg! 3
-  let e := Reify.reify (G'.getArg! 4)
+  let_expr subst_okR _ x v e E := G | return none
+  let .lit (.strVal x) := x | return none
+  let e := Reify.reify e
   let e' := (Reify.subst x v e).unreify
   let g' := {ig with goal := Expr.beta E #[e']}.toExpr
 --  let ⟨g', _⟩ ← goal.withContext (dsimpWithExt `irun_simp g')
@@ -671,12 +582,13 @@ def irunSubst : IRunTacticType := fun goal => do profileitM Exception "irunSubst
 
 end
 
-theorem expr_ok_test (P : Val -> PROP) :
-  ⊢ .inhale (.own (P (.nat 10))) ⇓ λ _ =>
-     expr_ok (.binop (.val (.nat 5)) .plus (.val (.nat 5))) ⇓ λ v =>
-     .exhale (.own (P v)) ⇓ λ _ =>
-     .done ⇓ ! := by
+theorem expr_okR_test (P : Val -> PROP) :
+  ⊢ (inhale (own (P (.nat 10)))).run λ _ =>
+     (expr_ok (.binop (.val (.nat 5)) .plus (.val (.nat 5)))).run λ v =>
+     (exhale (own (P v))).run λ _ =>
+     done.run empty := by
   istart
+  simp [irun_preprocess]
   irun 1
   irun 1
   irun 1
@@ -693,12 +605,13 @@ attribute [irun_simp] Nat.add_one_sub_one
 set_option profiler true in
 --set_option profiler.threshold 1 in
 #time theorem expr_ok_test2 (P : Val -> PROP) :
-   ⊢ .inhale (.own (P (.nat 0))) ⇓ λ _ =>
-      expr_ok (.app (.val rec_fn) (.val (.nat 200))) ⇓ λ v =>
-      .exhale (.own (P v)) ⇓ λ _ =>
-      .done ⇓ ! := by
+   ⊢ ((inhale (own (P (.nat 0)))) |>.bind λ _ =>
+      (expr_ok (.app (.val rec_fn) (.val (.nat 200)))) |>.bind λ v =>
+      (exhale (own (P v))) |>.bind λ _ =>
+      done).run empty := by
   istart
   unfold rec_fn
+  simp [irun_preprocess]
   --set_option trace.profiler true in
   --set_option trace.profiler.threshold 1 in
   --set_option diagnostics true in
